
\chapter{Mathematical Topics}
%
%
\section{Complex Numbers}
%
\[
    i = \sqrt{-1}
\]
Let $z=x+iy$

\medskip
\noindent
Complex conjugate:
\[
   \overline{z} = x-iy.
\]
Magnitude or modulus:
\[
   \| z \| = \sqrt{x^2+y^2}
\]
Note
\[
   z \overline{z} = x^2+y^2 = \| z \|^2
\]
\[
   \frac{1}{z} = \frac{\overline{z}}{\|z\|^2}
\]
Euler's formula\index{Euler's formula}
\begin{equation}
   e^{i\theta} = \cos\theta + i \sin\theta
   \label{eqn:EULER}
\end{equation}
%
\section{Geometric Sum, Geometric Series}
\index{geometric series}
\index{geometric sum}

\subsection*{Geometric Sum}
We derive the formula for the
geometric sum:
\begin{equation}
  \sum_{k=0}^{n} r^k = \frac{1- r^{n+1}}{1-r}.
\label{eqn:geometricsum}
\end{equation}

Let
\begin{equation}
  S = \sum_{k=0}^{n} r^k
\end{equation}
We multiply both sides by $r$, and then manipulate
the right side so that it is expressed in terms of $S$:
\begin{equation}
\begin{split}
  r S & = r \sum_{k=0}^{n}r^k \\
     & = \sum_{k=0}^{n}r^{k+1} \\
     & = \sum_{k=1}^{n+1}r^k \\
     & = r^{n+1} - 1 + \sum_{k=0}^{n}r^k \\
     & = r^{n+1} - 1 + S \\
\end{split}
\label{eqn:derivation}
\end{equation}
Now solve for $S$ to obtain
\begin{equation}
   S = \frac{1-r^{n+1}}{1-r} .
\end{equation}

\medskip
\noindent
If the starting index is $1$ instead of $0$,
we can derive a formula by using the previous
result:
\begin{equation}
\begin{split}
  \sum_{k=1}^{n} r^k & = \sum_{k=0}^{n-1}r^{k+1} \\
      & = r \sum_{k=0}^{n-1} r^{k} \\
      & = r\left(\frac{1-r^n}{1-r}\right).
\end{split}
\label{eqn:geomsumfromone}
\end{equation}
% \begin{question}
% Derive this result by using the same method as in
% Equation~\eqref{eqn:derivation}.
% \end{question}

\subsection*{Geometric Series.}
If $0 < r < 1$, then
\begin{equation}
   \sum_{k=0}^{\infty} r^k = \frac{1}{1-r}
\end{equation}
\noindent
\emph{Proof.}
\[
  \sum_{k=0}^{\infty} r^k
    = \lim_{n\rightarrow\infty} \sum_{k=0}^{n} r^n
    = \lim_{n\rightarrow\infty} \frac{1-r^{n+1}}{1-r}
    = \frac{1}{1-r}.
\]
%
\section{Cobb-Douglas Function}
%
\label{sec:cobbdouglas}
A function that often arises in economics
is the \emph{Cobb-Douglas function}:\index{Cobb-Douglas function}
\begin{equation}
  f(x,y) = cx^{\alpha}y^{\beta}
\end{equation}
When $\alpha+\beta=1$, the function is said to have
\emph{constant returns to scale},\index{constant returns to scale}
and in this case it may
be written
\begin{equation}
  f(x,y) = cx^{\alpha}y^{1-\alpha}
\end{equation}
The mathematical term for \emph{constant returns to scale}
is \emph{linearly homogeneous}.\index{homogeneous, linearly}
It is easy to verify:
\begin{equation}
  f(kx,ky) = c(kx)^{\alpha}(ky)^{1-\alpha}
     = k^{\alpha}k^{1-\alpha} c x^{\alpha}y^{1-\alpha}
     = k c x^{\alpha}y^{1-\alpha}
     = k f(x,y).
\end{equation}
%
\section{A Few Calculus Reminders}

A function $f$ is \emph{continuous}\index{continuous} at at point $a$ if
\[
  \lim_{x\rightarrow a} f(x) = f(a).
\]
%
We say $f$ is \emph{continuous on the interval} $(a,b)$ if
$f$ is continuous at each point in the interval.
%
\section{Partial Derivatives}
\label{sec:PartialDerivs}
The \emph{partial derivative of $f(x,y)$ with respect to $x$},
written $f_x(x,y)$ or $\frac{\partial f}{\partial x}$, is
defined to be
\[
   f_x(x,y) = \lim_{h\rightarrow 0} \frac{f(x+h,y)}{h}.
\]
There is a corresponding definition for $f_y(x,y)$,
and the generalizations to more variables
(such as $f_y(w,x,y,z)$) should be clear.
